workloads/Coq/RBT/Runners/BespokeGenerator_test_runner.v
@@ -25,9 +25,9 @@ fun test_name ->
   let test = List.assoc test_name test_map in
   test ()
 
-
 let () =
-  Sys.argv.(1) |> qctest_map
+Sys.argv.(1) |> qctest_map
+
 ".
 
 Extraction "BespokeGenerator_test_runner.ml" qctest_test_prop_InsertValid qctest_test_prop_DeleteValid qctest_test_prop_InsertPost qctest_test_prop_DeletePost qctest_test_prop_InsertModel qctest_test_prop_DeleteModel qctest_test_prop_InsertInsert qctest_test_prop_InsertDelete qctest_test_prop_DeleteInsert qctest_test_prop_DeleteDelete qctest_map.
