workloads/Coq/RBT/Runners/TypeBasedFuzzer_test_runner.v
@@ -1,6 +1,7 @@
 From RBT Require Import TypeBasedFuzzer.
 From QuickChick Require Import QuickChick.
 Set Warnings "-extraction-opaque-accessed,-extraction".
+Axiom num_tests : nat. Extract Constant num_tests => "max_int".
 Definition qctest_test_prop_InsertValid := (fun _ : unit => print_extracted_coq_string ("[|{" ++ show (withTime (fun tt => (test_prop_InsertValid_fuzzer tt))) ++ "}|]")).
 Definition qctest_test_prop_DeleteValid := (fun _ : unit => print_extracted_coq_string ("[|{" ++ show (withTime (fun tt => (test_prop_DeleteValid_fuzzer tt))) ++ "}|]")).
 Definition qctest_test_prop_InsertPost := (fun _ : unit => print_extracted_coq_string ("[|{" ++ show (withTime (fun tt => (test_prop_InsertPost_fuzzer tt))) ++ "}|]")).
@@ -24,11 +25,11 @@ fun test_name ->
   let test = List.assoc test_name test_map in
   test ()
 
-
-let () = 
+let () =
   Printf.printf ""Entering main of qc_exec\n""; flush stdout;
   setup_shm_aux ();
   Sys.argv.(1) |> qctest_map ; flush stdout;
+
 ".
 
 Extraction "TypeBasedFuzzer_test_runner.ml" qctest_test_prop_InsertValid qctest_test_prop_DeleteValid qctest_test_prop_InsertPost qctest_test_prop_DeletePost qctest_test_prop_InsertModel qctest_test_prop_DeleteModel qctest_test_prop_InsertInsert qctest_test_prop_InsertDelete qctest_test_prop_DeleteInsert qctest_test_prop_DeleteDelete qctest_map.
