workloads/Coq/RBTProplang/Runners/TypeBasedGenerator_test_runner.v
@@ -2,16 +2,16 @@ From RBTProplang Require Import TypeBasedGenerator.
 From QuickChick Require Import QuickChick.
 Set Warnings "-extraction-opaque-accessed,-extraction".
 Axiom num_tests : nat. Extract Constant num_tests => "max_int".
-Definition qctest_test_prop_InsertValid_runner := (fun _ : unit => print_extracted_coq_string ("[|{" ++ show (withTime(fun tt => (sample1 test_prop_InsertValid_runner))) ++ "}|]")).
-Definition qctest_test_prop_DeleteValid_runner := (fun _ : unit => print_extracted_coq_string ("[|{" ++ show (withTime(fun tt => (sample1 test_prop_DeleteValid_runner))) ++ "}|]")).
-Definition qctest_test_prop_InsertPost_runner := (fun _ : unit => print_extracted_coq_string ("[|{" ++ show (withTime(fun tt => (sample1 test_prop_InsertPost_runner))) ++ "}|]")).
-Definition qctest_test_prop_DeletePost_runner := (fun _ : unit => print_extracted_coq_string ("[|{" ++ show (withTime(fun tt => (sample1 test_prop_DeletePost_runner))) ++ "}|]")).
-Definition qctest_test_prop_InsertModel_runner := (fun _ : unit => print_extracted_coq_string ("[|{" ++ show (withTime(fun tt => (sample1 test_prop_InsertModel_runner))) ++ "}|]")).
-Definition qctest_test_prop_DeleteModel_runner := (fun _ : unit => print_extracted_coq_string ("[|{" ++ show (withTime(fun tt => (sample1 test_prop_DeleteModel_runner))) ++ "}|]")).
-Definition qctest_test_prop_InsertInsert_runner := (fun _ : unit => print_extracted_coq_string ("[|{" ++ show (withTime(fun tt => (sample1 test_prop_InsertInsert_runner))) ++ "}|]")).
-Definition qctest_test_prop_InsertDelete_runner := (fun _ : unit => print_extracted_coq_string ("[|{" ++ show (withTime(fun tt => (sample1 test_prop_InsertDelete_runner))) ++ "}|]")).
-Definition qctest_test_prop_DeleteInsert_runner := (fun _ : unit => print_extracted_coq_string ("[|{" ++ show (withTime(fun tt => (sample1 test_prop_DeleteInsert_runner))) ++ "}|]")).
-Definition qctest_test_prop_DeleteDelete_runner := (fun _ : unit => print_extracted_coq_string ("[|{" ++ show (withTime(fun tt => (sample1 test_prop_DeleteDelete_runner))) ++ "}|]")).
+Definition qctest_test_prop_InsertValid := (fun _ : unit => print_extracted_coq_string ("[|{" ++ show (withTime(fun tt => (sample1 test_prop_InsertValid))) ++ "}|]")).
+Definition qctest_test_prop_DeleteValid := (fun _ : unit => print_extracted_coq_string ("[|{" ++ show (withTime(fun tt => (sample1 test_prop_DeleteValid))) ++ "}|]")).
+Definition qctest_test_prop_InsertPost := (fun _ : unit => print_extracted_coq_string ("[|{" ++ show (withTime(fun tt => (sample1 test_prop_InsertPost))) ++ "}|]")).
+Definition qctest_test_prop_DeletePost := (fun _ : unit => print_extracted_coq_string ("[|{" ++ show (withTime(fun tt => (sample1 test_prop_DeletePost))) ++ "}|]")).
+Definition qctest_test_prop_InsertModel := (fun _ : unit => print_extracted_coq_string ("[|{" ++ show (withTime(fun tt => (sample1 test_prop_InsertModel))) ++ "}|]")).
+Definition qctest_test_prop_DeleteModel := (fun _ : unit => print_extracted_coq_string ("[|{" ++ show (withTime(fun tt => (sample1 test_prop_DeleteModel))) ++ "}|]")).
+Definition qctest_test_prop_InsertInsert := (fun _ : unit => print_extracted_coq_string ("[|{" ++ show (withTime(fun tt => (sample1 test_prop_InsertInsert))) ++ "}|]")).
+Definition qctest_test_prop_InsertDelete := (fun _ : unit => print_extracted_coq_string ("[|{" ++ show (withTime(fun tt => (sample1 test_prop_InsertDelete))) ++ "}|]")).
+Definition qctest_test_prop_DeleteInsert := (fun _ : unit => print_extracted_coq_string ("[|{" ++ show (withTime(fun tt => (sample1 test_prop_DeleteInsert))) ++ "}|]")).
+Definition qctest_test_prop_DeleteDelete := (fun _ : unit => print_extracted_coq_string ("[|{" ++ show (withTime(fun tt => (sample1 test_prop_DeleteDelete))) ++ "}|]")).
 
 
 Parameter OCamlString : Type.
@@ -20,7 +20,7 @@ Axiom qctest_map : OCamlString -> unit.
 Extract Constant qctest_map => "
 fun test_name ->
   let test_map = [
-    (""test_prop_InsertValid_runner"", qctest_test_prop_InsertValid_runner); (""test_prop_DeleteValid_runner"", qctest_test_prop_DeleteValid_runner); (""test_prop_InsertPost_runner"", qctest_test_prop_InsertPost_runner); (""test_prop_DeletePost_runner"", qctest_test_prop_DeletePost_runner); (""test_prop_InsertModel_runner"", qctest_test_prop_InsertModel_runner); (""test_prop_DeleteModel_runner"", qctest_test_prop_DeleteModel_runner); (""test_prop_InsertInsert_runner"", qctest_test_prop_InsertInsert_runner); (""test_prop_InsertDelete_runner"", qctest_test_prop_InsertDelete_runner); (""test_prop_DeleteInsert_runner"", qctest_test_prop_DeleteInsert_runner); (""test_prop_DeleteDelete_runner"", qctest_test_prop_DeleteDelete_runner)
+    (""test_prop_InsertValid"", qctest_test_prop_InsertValid); (""test_prop_DeleteValid"", qctest_test_prop_DeleteValid); (""test_prop_InsertPost"", qctest_test_prop_InsertPost); (""test_prop_DeletePost"", qctest_test_prop_DeletePost); (""test_prop_InsertModel"", qctest_test_prop_InsertModel); (""test_prop_DeleteModel"", qctest_test_prop_DeleteModel); (""test_prop_InsertInsert"", qctest_test_prop_InsertInsert); (""test_prop_InsertDelete"", qctest_test_prop_InsertDelete); (""test_prop_DeleteInsert"", qctest_test_prop_DeleteInsert); (""test_prop_DeleteDelete"", qctest_test_prop_DeleteDelete)
   ] in
   let test = List.assoc test_name test_map in
   test ()
@@ -30,4 +30,4 @@ Sys.argv.(1) |> qctest_map
 
 ".
 
-Extraction "TypeBasedGenerator_test_runner.ml" qctest_test_prop_InsertValid_runner qctest_test_prop_DeleteValid_runner qctest_test_prop_InsertPost_runner qctest_test_prop_DeletePost_runner qctest_test_prop_InsertModel_runner qctest_test_prop_DeleteModel_runner qctest_test_prop_InsertInsert_runner qctest_test_prop_InsertDelete_runner qctest_test_prop_DeleteInsert_runner qctest_test_prop_DeleteDelete_runner qctest_map.
+Extraction "TypeBasedGenerator_test_runner.ml" qctest_test_prop_InsertValid qctest_test_prop_DeleteValid qctest_test_prop_InsertPost qctest_test_prop_DeletePost qctest_test_prop_InsertModel qctest_test_prop_DeleteModel qctest_test_prop_InsertInsert qctest_test_prop_InsertDelete qctest_test_prop_DeleteInsert qctest_test_prop_DeleteDelete qctest_map.
