workloads/Coq/RBTProplang/Strategies/TypeBasedGenerator.v
@@ -15,6 +15,7 @@ From RBTProplang Require Import Impl Spec.
 From PropLang Require Import PropLang.
 
 Local Open Scope prop_scope.
+Open Scope Z_scope.
 
 (* --------------------- Generator --------------------- *)
 
@@ -30,110 +31,166 @@ Extract Constant number_of_trials => "max_int".
 
 (* --------------------- Tests --------------------- *)
 
-Definition test_prop_InsertValid   :=
-	@ForAll _ ∅ _ "t" (fun tt => arbitrary) (fun tt n => (fun n => arbitrary)) (fun tt n => shrink n) (fun tt n => show n) (
-	@ForAll _ (Tree · ∅) _ "k" (fun '(t, tt) => arbitrary) (fun '(t, tt) n => (fun n => arbitrary)) (fun '(t, tt) n => shrink n) (fun '(t, tt) n => show n) (
-	@ForAll _ (Z · (Tree · ∅)) _ "v" (fun '(k, (t, tt)) => arbitrary) (fun '(k, (t, tt)) n => (fun n => arbitrary)) (fun '(k, (t, tt)) n => shrink n) (fun '(k, (t, tt)) n => show n) (
-	@Predicate (Z · (Z · (Tree · ∅))) Z
-	(fun '(v, (k, (t, tt))) => (prop_InsertValid t k v, 0%Z))))).
 
-Definition test_prop_InsertValid_runner := (runLoop number_of_trials test_prop_InsertValid).
+Definition prop_InsertValid :=
+	ForAll "t" (fun tt => arbitrary) (fun tt t => arbitrary) (fun tt => shrink) (fun tt => show) (
+	Implies (Tree · ∅) "isRBT t" (fun '(t, tt) => isRBT t) (
+	ForAll "k" (fun tt => arbitrary) (fun tt k => arbitrary) (fun tt => shrink) (fun tt => show) (
+	ForAll "v" (fun tt => arbitrary) (fun tt v => arbitrary) (fun tt => shrink) (fun tt => show) (
+	Check (Z · (Z · (Tree · ∅)))
+	(fun '(v, (k, (t, tt))) => (isRBT (insert k v t))))))).
 
-(*! QuickProp test_prop_InsertValid_runner. *)
+Definition test_prop_InsertValid := (runLoop number_of_trials prop_InsertValid).
+(*! QuickProp test_prop_InsertValid. *)
 
-Definition test_prop_DeleteValid   :=
-	@ForAll _ ∅ _ "t" (fun tt => arbitrary) (fun tt n => (fun n => arbitrary)) (fun tt n => shrink n) (fun tt n => show n) (
-	@ForAll _ (Tree · ∅) _ "k" (fun '(t, tt) => arbitrary) (fun '(t, tt) n => (fun n => arbitrary)) (fun '(t, tt) n => shrink n) (fun '(t, tt) n => show n) (
-	@Predicate (Z · (Tree · ∅)) Z
-	(fun '(k, (t, tt)) => (prop_DeleteValid t k, 0%Z)))).
+Definition prop_DeleteValid :=
+	ForAll "t" (fun tt => arbitrary) (fun tt t => arbitrary) (fun tt => shrink) (fun tt => show) (
+	Implies (Tree · ∅) "isRBT t" (fun '(t, tt) => isRBT t) (
+	ForAll "k" (fun tt => arbitrary) (fun tt n => arbitrary) (fun tt => shrink) (fun tt => show) (
+	Check (Z · (Tree · ∅))
+	(fun '(k, (t, tt)) => (match delete k t with
+						   | None => false
+						   | Some t' => isRBT t'
+							end))))).
 
-Definition test_prop_DeleteValid_runner := (runLoop number_of_trials test_prop_DeleteValid).
+Definition test_prop_DeleteValid := (runLoop number_of_trials prop_DeleteValid).
+(*! QuickProp test_prop_DeleteValid. *)
 
-(*! QuickProp test_prop_DeleteValid_runner. *)
+Definition prop_InsertPost :=
+	ForAll "t" (fun tt => arbitrary) (fun tt t => arbitrary) (fun tt => shrink) (fun tt => show) (
+	Implies (Tree · ∅) "isRBT t" (fun '(t, tt) => isRBT t) (
+	ForAll "k" (fun tt => arbitrary) (fun tt k => arbitrary) (fun tt => shrink) (fun tt => show) (
+	ForAll "k'" (fun tt => arbitrary) (fun tt k' => arbitrary) (fun tt => shrink) (fun tt => show) (
+	ForAll "v" (fun tt => arbitrary) (fun tt v => arbitrary) (fun tt => shrink) (fun tt => show) (
+	Check (Z · (Z · (Z · (Tree · ∅))))
+	(fun '(v, (k', (k, (t, tt)))) => (let v' := find k' (insert k v t) in
+										if k =? k' then v' ==? Some v 
+										else v' ==? find k' t))))))).
 
-Definition test_prop_InsertPost    :=
-	@ForAll _ ∅ _ "t" (fun tt => arbitrary) (fun tt n => (fun n => arbitrary)) (fun tt n => shrink n) (fun tt n => show n) (
-	@ForAll _ (Tree · ∅) _ "k" (fun '(t, tt) => arbitrary) (fun '(t, tt) n => (fun n => arbitrary)) (fun '(t, tt) n => shrink n) (fun '(t, tt) n => show n) (
-	@ForAll _ (Z · (Tree · ∅)) _ "k'" (fun '(k, (t, tt)) => arbitrary) (fun '(k, (t, tt)) n => (fun n => arbitrary)) (fun '(k, (t, tt)) n => shrink n) (fun '(k, (t, tt)) n => show n) (
-	@ForAll _ (Z · (Z · (Tree · ∅))) _ "v" (fun '(k', (k, (t, tt))) => arbitrary) (fun '(k', (k, (t, tt))) n => (fun n => arbitrary)) (fun '(k', (k, (t, tt))) n => shrink n) (fun '(k', (k, (t, tt))) n => show n) (
-	@Predicate (Z · (Z · (Z · (Tree · ∅)))) Z
-	(fun '(v, (k', (k, (t, tt)))) => (prop_InsertPost t k k' v, 0%Z)))))).
+Definition test_prop_InsertPost := (runLoop number_of_trials prop_InsertPost).
+(*! QuickProp test_prop_InsertPost. *)
 
-Definition test_prop_InsertPost_runner := (runLoop number_of_trials test_prop_InsertPost).
-(*! QuickProp test_prop_InsertPost_runner. *)
+Definition prop_DeletePost :=
+	ForAll "t" (fun tt => arbitrary) (fun tt t => arbitrary) (fun tt => shrink) (fun tt => show) (
+	Implies (Tree · ∅) "isRBT t" (fun '(t, tt) => isRBT t) (
+	ForAll "k" (fun tt => arbitrary) (fun tt t => arbitrary) (fun tt => shrink) (fun tt => show) (
+	ForAll "k'" (fun tt => arbitrary) (fun tt n => arbitrary) (fun tt => shrink) (fun tt => show) (
+	Check (Z · (Z · (Tree · ∅)))
+	(fun '(k', (k, (t, tt))) => (t' <- delete k t ;;
+								 find k' t' ==? if k =? k' then None else find k' t)))))).
 
-Definition test_prop_DeletePost    :=
-	@ForAll _ ∅ _ "t" (fun tt => arbitrary) (fun tt n => (fun n => arbitrary)) (fun tt n => shrink n) (fun tt n => show n) (
-	@ForAll _ (Tree · ∅) _ "k" (fun '(t, tt) => arbitrary) (fun '(t, tt) n => (fun n => arbitrary)) (fun '(t, tt) n => shrink n) (fun '(t, tt) n => show n) (
-	@ForAll _ (Z · (Tree · ∅)) _ "k'" (fun '(k, (t, tt)) => arbitrary) (fun '(k, (t, tt)) n => (fun n => arbitrary)) (fun '(k, (t, tt)) n => shrink n) (fun '(k, (t, tt)) n => show n) (
-	@Predicate (Z · (Z · (Tree · ∅))) Z
-	(fun '(k', (k, (t, tt))) => (prop_DeletePost t k k', 0%Z))))).
-
-Definition test_prop_DeletePost_runner := (runLoop number_of_trials test_prop_DeletePost).
-(*! QuickProp test_prop_DeletePost_runner. *)
-
-Definition test_prop_InsertModel    :=
-	@ForAll _ ∅ _ "t" (fun tt => arbitrary) (fun tt n => (fun n => arbitrary)) (fun tt n => shrink n) (fun tt n => show n) (
-	@ForAll _ (Tree · ∅) _ "k" (fun '(t, tt) => arbitrary) (fun '(t, tt) n => (fun n => arbitrary)) (fun '(t, tt) n => shrink n) (fun '(t, tt) n => show n) (
-	@ForAll _ (Z · (Tree · ∅)) _ "v'" (fun '(v, (t, tt)) => arbitrary) (fun '(v, (t, tt)) n => (fun n => arbitrary)) (fun '(v, (t, tt)) n => shrink n) (fun '(v, (t, tt)) n => show n) (
-	@Predicate (Z · (Z · (Tree · ∅))) Z
-	(fun '(v, (k, (t, tt))) => (prop_InsertModel t k v, 0%Z))))).
-
-    
-Definition test_prop_InsertModel_runner := (runLoop number_of_trials test_prop_InsertModel).
-(*! QuickProp test_prop_InsertModel_runner. *)
-
-Definition test_prop_DeleteModel    :=
-	@ForAll _ ∅ _ "t" (fun tt => arbitrary) (fun tt n => (fun n => arbitrary)) (fun tt n => shrink n) (fun tt n => show n) (
-	@ForAll _ (Tree · ∅) _ "k" (fun '(t, tt) => arbitrary) (fun '(t, tt) n => (fun n => arbitrary)) (fun '(t, tt) n => shrink n) (fun '(t, tt) n => show n) (
-	@Predicate (Z · (Tree · ∅)) Z
-	(fun '(k, (t, tt)) => (prop_DeleteModel t k, 0%Z)))).
-
-    
-Definition test_prop_DeleteModel_runner := (runLoop number_of_trials test_prop_DeleteModel).
-(*! QuickProp test_prop_DeleteModel_runner. *)
-
-Definition test_prop_InsertInsert    :=
-	@ForAll _ ∅ _ "t" (fun tt => arbitrary) (fun tt n => (fun n => arbitrary)) (fun tt n => shrink n) (fun tt n => show n) (
-	@ForAll _ (Tree · ∅) _ "k" (fun '(t, tt) => arbitrary) (fun '(t, tt) n => (fun n => arbitrary)) (fun '(t, tt) n => shrink n) (fun '(t, tt) n => show n) (
-	@ForAll _ (Z · (Tree · ∅)) _ "k'" (fun '(k, (t, tt)) => arbitrary) (fun '(k, (t, tt)) n => (fun n => arbitrary)) (fun '(k, (t, tt)) n => shrink n) (fun '(k, (t, tt)) n => show n) (
-	@ForAll _ (Z · (Z · (Tree · ∅))) _ "v" (fun '(k', (k, (t, tt))) => arbitrary) (fun '(k', (k, (t, tt))) n => (fun n => arbitrary)) (fun '(k', (k, (t, tt))) n => shrink n) (fun '(k', (k, (t, tt))) n => show n) (
-	@ForAll _ (Z · (Z · (Z · (Tree · ∅)))) _ "v'" (fun '(v, (k', (k, (t, tt)))) => arbitrary) (fun '(v, (k', (k, (t, tt)))) n => (fun n => arbitrary)) (fun '(v, (k', (k, (t, tt)))) n => shrink n) (fun '(v, (k', (k, (t, tt)))) n => show n) (
-	@Predicate (Z · (Z · (Z · (Z · (Tree · ∅))))) Z
-	(fun '(v', (v, (k', (k, (t, tt))))) => (prop_InsertInsert t k k' v v', 0%Z))))))).
-
-Definition test_prop_InsertInsert_runner := (runLoop number_of_trials test_prop_InsertInsert).
-(*! QuickProp test_prop_InsertInsert_runner. *)
-
-Definition test_prop_InsertDelete    :=
-	@ForAll _ ∅ _ "t" (fun tt => arbitrary) (fun tt n => (fun n => arbitrary)) (fun tt n => shrink n) (fun tt n => show n) (
-	@ForAll _ (Tree · ∅) _ "k" (fun '(t, tt) => arbitrary) (fun '(t, tt) n => (fun n => arbitrary)) (fun '(t, tt) n => shrink n) (fun '(t, tt) n => show n) (
-	@ForAll _ (Z · (Tree · ∅)) _ "k'" (fun '(k, (t, tt)) => arbitrary) (fun '(k, (t, tt)) n => (fun n => arbitrary)) (fun '(k, (t, tt)) n => shrink n) (fun '(k, (t, tt)) n => show n) (
-	@ForAll _ (Z · (Z · (Tree · ∅))) _ "v" (fun '(k', (k, (t, tt))) => arbitrary) (fun '(k', (k, (t, tt))) n => (fun n => arbitrary)) (fun '(k', (k, (t, tt))) n => shrink n) (fun '(k', (k, (t, tt))) n => show n) (
-	@Predicate (Z · (Z · (Z · (Tree · ∅)))) Z
-	(fun '(v, (k', (k, (t, tt)))) => (prop_InsertDelete t k k' v, 0%Z)))))).
-
-Definition test_prop_InsertDelete_runner := (runLoop number_of_trials test_prop_InsertDelete).
-(*! QuickProp test_prop_InsertDelete_runner. *)
+Definition test_prop_DeletePost := (runLoop number_of_trials prop_DeletePost).
+(*! QuickProp test_prop_DeletePost. *)
 
 
-Definition test_prop_DeleteInsert    :=
-	@ForAll _ ∅ _ "t" (fun tt => arbitrary) (fun tt n => (fun n => arbitrary)) (fun tt n => shrink n) (fun tt n => show n) (
-	@ForAll _ (Tree · ∅) _ "k" (fun '(t, tt) => arbitrary) (fun '(t, tt) n => (fun n => arbitrary)) (fun '(t, tt) n => shrink n) (fun '(t, tt) n => show n) (
-	@ForAll _ (Z · (Tree · ∅)) _ "k'" (fun '(k, (t, tt)) => arbitrary) (fun '(k, (t, tt)) n => (fun n => arbitrary)) (fun '(k, (t, tt)) n => shrink n) (fun '(k, (t, tt)) n => show n) (
-	@ForAll _ (Z · (Z · (Tree · ∅))) _ "v'" (fun '(k', (k, (t, tt))) => arbitrary) (fun '(k', (k, (t, tt))) n => (fun n => arbitrary)) (fun '(k', (k, (t, tt))) n => shrink n) (fun '(k', (k, (t, tt))) n => show n) (
-	@Predicate (Z · (Z · (Z · (Tree · ∅)))) Z
-	(fun '(v', (k', (k, (t, tt)))) => (prop_DeleteInsert t k k' v', 0%Z)))))).
+Definition prop_InsertModel :=
+	ForAll "t" (fun tt => arbitrary) (fun tt t => arbitrary) (fun tt => shrink) (fun tt => show) (
+	Implies (Tree · ∅) "isRBT t" (fun '(t, tt) => isRBT t) (
+	ForAll "k" (fun tt => arbitrary) (fun tt t => arbitrary) (fun tt => shrink) (fun tt => show) (
+	ForAll "v" (fun tt => arbitrary) (fun tt n => arbitrary) (fun tt => shrink) (fun tt => show) (
+	Check (Z · (Z · (Tree · ∅)))
+	(fun '(v, (k, (t, tt))) => ((toList (insert k v t) = L_insert (k, v) (deleteKey k (toList t)))?)))))).
 
-Definition test_prop_DeleteInsert_runner := (runLoop number_of_trials test_prop_DeleteInsert).
-(*! QuickProp test_prop_DeleteInsert_runner. *)
+Definition test_prop_InsertModel := (runLoop number_of_trials prop_InsertModel).
+(*! QuickProp test_prop_InsertModel. *)
 
-Definition test_prop_DeleteDelete    :=
-	@ForAll _ ∅ _ "t" (fun tt => arbitrary) (fun tt n => (fun n => arbitrary)) (fun tt n => shrink n) (fun tt n => show n) (
-	@ForAll _ (Tree · ∅) _ "k" (fun '(t, tt) => arbitrary) (fun '(t, tt) n => (fun n => arbitrary)) (fun '(t, tt) n => shrink n) (fun '(t, tt) n => show n) (
-	@ForAll _ (Z · (Tree · ∅)) _ "k'" (fun '(k, (t, tt)) => arbitrary) (fun '(k, (t, tt)) n => (fun n => arbitrary)) (fun '(k, (t, tt)) n => shrink n) (fun '(k, (t, tt)) n => show n) (
-	@Predicate (Z · (Z · (Tree · ∅))) Z
-	(fun '(k', (k, (t, tt))) => ((prop_DeleteDelete t k k', 0%Z)))))).
+Definition prop_DeleteModel :=
+	ForAll "t" (fun tt => arbitrary) (fun tt t => arbitrary) (fun tt => shrink) (fun tt => show) (
+	Implies (Tree · ∅) "isRBT t" (fun '(t, tt) => isRBT t) (
+	ForAll "k" (fun tt => arbitrary) (fun tt t => arbitrary) (fun tt => shrink) (fun tt => show) (
+	Check (Z · (Tree · ∅))
+	(fun '(k, (t, tt)) => ( match delete k t with
+							| None => false
+							| Some t' => (toList t' = deleteKey k (toList t))?
+							end))))).
 
-Definition test_prop_DeleteDelete_runner := (runLoop number_of_trials test_prop_DeleteDelete).
-(*! QuickProp test_prop_DeleteDelete_runner. *)
+Definition test_prop_DeleteModel := (runLoop number_of_trials prop_DeleteModel).
+(*! QuickProp test_prop_DeleteModel. *)
+
+Definition prop_InsertInsert :=
+	ForAll "t" (fun tt => arbitrary) (fun tt t => arbitrary) (fun tt => shrink) (fun tt => show) (
+	Implies (Tree · ∅) "isRBT t" (fun '(t, tt) => isRBT t) (
+	ForAll "k" (fun tt => arbitrary) (fun tt t => arbitrary) (fun tt => shrink) (fun tt => show) (
+	ForAll "k'" (fun tt => arbitrary) (fun tt n => arbitrary) (fun tt => shrink) (fun tt => show) (
+	ForAll "v" (fun tt => arbitrary) (fun tt v => arbitrary) (fun tt => shrink) (fun tt => show) (
+	ForAll "v'" (fun tt => arbitrary) (fun tt v' => arbitrary) (fun tt => shrink) (fun tt => show) (
+	Check (Z · (Z · (Z · (Z · (Tree · ∅)))))
+	(fun '(v', (v, (k', (k, (t, tt))))) => ((toList (insert k v (insert k' v' t))
+    ==? toList(if k =? k' then insert k v t else insert k' v' (insert k v t))))))))))).
+
+Definition test_prop_InsertInsert := (runLoop number_of_trials prop_InsertInsert).
+(*! QuickProp test_prop_InsertInsert. *)
+
+
+Definition prop_InsertDelete :=
+	ForAll "t" (fun tt => arbitrary) (fun tt t => arbitrary) (fun tt => shrink) (fun tt => show) (
+	Implies (Tree · ∅) "isRBT t" (fun '(t, tt) => isRBT t) (
+	ForAll "k" (fun tt => arbitrary) (fun tt k => arbitrary) (fun tt => shrink) (fun tt => show) (
+	ForAll "k'" (fun tt => arbitrary) (fun tt k' => arbitrary) (fun tt => shrink) (fun tt => show) (
+	ForAll "v" (fun tt => arbitrary) (fun tt v => arbitrary) (fun tt => shrink) (fun tt => show) (
+	Check (Z · (Z · (Z · (Tree · ∅))))
+	(fun '(v, (k', (k, (t, tt)))) => (
+		match (delete k' t) with
+		| None => false
+		| Some t' =>
+			match delete k' (insert k v t) with
+			| None => false
+			| Some t'' =>
+				toList(insert k v t') ==? toList(if k =? k' then insert k v t else t'')
+			end
+		end))))))).
+
+Definition test_prop_InsertDelete := (runLoop number_of_trials prop_InsertDelete).
+(*! QuickProp test_prop_InsertDelete. *)
+
+Definition prop_DeleteInsert :=
+	ForAll "t" (fun tt => arbitrary) (fun tt t => arbitrary) (fun tt => shrink) (fun tt => show) (
+	Implies (Tree · ∅) "isRBT t" (fun '(t, tt) => isRBT t) (
+	ForAll "k" (fun tt => arbitrary) (fun tt t => arbitrary) (fun tt => shrink) (fun tt => show) (
+	ForAll "k'" (fun tt => arbitrary) (fun tt n => arbitrary) (fun tt => shrink) (fun tt => show) (
+	ForAll "v'" (fun tt => arbitrary) (fun tt v => arbitrary) (fun tt => shrink) (fun tt => show) (
+	Check (Z · (Z · (Z · (Tree · ∅))))
+	(fun '(v', (k', (k, (t, tt)))) => (
+		match delete k (insert k' v' t) with
+		| None => false
+		| Some t' =>
+		  match delete k t with
+		  | None => false
+		  | Some t'' =>
+			let t''' := insert k' v' t'' in
+			toList t' ==? toList (if k =? k' then t'' else t''')
+		  end
+		end
+	))))))).
+
+Definition test_prop_DeleteInsert := (runLoop number_of_trials prop_DeleteInsert).
+(*! QuickProp test_prop_DeleteInsert. *)
+
+Definition prop_DeleteDelete :=
+	ForAll "t" (fun tt => arbitrary) (fun tt t => arbitrary) (fun tt => shrink) (fun tt => show) (
+	Implies (Tree · ∅) "isRBT t" (fun '(t, tt) => isRBT t) (
+	ForAll "k" (fun tt => arbitrary) (fun tt t => arbitrary) (fun tt => shrink) (fun tt => show) (
+	ForAll "k'" (fun tt => arbitrary) (fun tt n => arbitrary) (fun tt => shrink) (fun tt => show) (
+	Check (Z · (Z · (Tree · ∅)))
+	(fun '(k', (k, (t, tt))) => (
+		match delete k' t with
+		| None => false
+		| Some t' =>
+		  match delete k t' with
+		  | None => false
+		  | Some t'' =>
+			match delete k t with
+			| None => false
+			| Some t1' =>
+			  match delete k' t1' with
+			  | None => false
+			  | Some t1'' =>
+				toList t'' ==? toList t1''
+			  end
+			end
+		  end
+		end
+	)))))).
+
+Definition test_prop_DeleteDelete := (runLoop number_of_trials prop_DeleteDelete).
+(*! QuickProp test_prop_DeleteDelete. *)
