workloads/Coq/STLCProplang/Runners/TypeBasedGenerator_test_runner.v
@@ -2,8 +2,8 @@ From STLCProplang Require Import TypeBasedGenerator.
 From QuickChick Require Import QuickChick.
 Set Warnings "-extraction-opaque-accessed,-extraction".
 Axiom num_tests : nat. Extract Constant num_tests => "max_int".
-Definition qctest_test_prop_SinglePreserve_runner := (fun _ : unit => print_extracted_coq_string ("[|{" ++ show (withTime(fun tt => (sample1 test_prop_SinglePreserve_runner))) ++ "}|]")).
-Definition qctest_test_prop_MultiPreserve_runner := (fun _ : unit => print_extracted_coq_string ("[|{" ++ show (withTime(fun tt => (sample1 test_prop_MultiPreserve_runner))) ++ "}|]")).
+Definition qctest_test_prop_SinglePreserve := (fun _ : unit => print_extracted_coq_string ("[|{" ++ show (withTime(fun tt => (sample1 test_prop_SinglePreserve))) ++ "}|]")).
+Definition qctest_test_prop_MultiPreserve := (fun _ : unit => print_extracted_coq_string ("[|{" ++ show (withTime(fun tt => (sample1 test_prop_MultiPreserve))) ++ "}|]")).
 
 
 Parameter OCamlString : Type.
@@ -12,7 +12,7 @@ Axiom qctest_map : OCamlString -> unit.
 Extract Constant qctest_map => "
 fun test_name ->
   let test_map = [
-    (""test_prop_SinglePreserve_runner"", qctest_test_prop_SinglePreserve_runner); (""test_prop_MultiPreserve_runner"", qctest_test_prop_MultiPreserve_runner)
+    (""test_prop_SinglePreserve"", qctest_test_prop_SinglePreserve); (""test_prop_MultiPreserve"", qctest_test_prop_MultiPreserve)
   ] in
   let test = List.assoc test_name test_map in
   test ()
@@ -22,4 +22,4 @@ Sys.argv.(1) |> qctest_map
 
 ".
 
-Extraction "TypeBasedGenerator_test_runner.ml" qctest_test_prop_SinglePreserve_runner qctest_test_prop_MultiPreserve_runner qctest_map.
+Extraction "TypeBasedGenerator_test_runner.ml" qctest_test_prop_SinglePreserve qctest_test_prop_MultiPreserve qctest_map.
