workloads/Coq/STLCProplang/Strategies/BespokeGenerator.v
@@ -111,125 +111,30 @@ Extract Constant number_of_trials => "max_int".
 
 (* --------------------- Tests --------------------- *)
 
-Definition test_prop_SinglePreserve   :=
-	@ForAllMaybe _ ∅ _ "e" (fun tt => gSized) (fun tt n => (fun n => gSized)) (fun tt n => shrink n) (fun tt n => show n) (
-	@Predicate (Expr · ∅) Z
-	(fun '(e, tt) => (prop_SinglePreserve e, 0%Z))).
+Definition prop_SinglePreserve   :=
+	ForAllMaybe "e" (fun tt => gSized) (fun tt e => gSized) (fun tt => shrink) (fun tt => show) (
+  Implies (Expr · ∅) "isJust (mt e)" (fun '(e, tt) => isJust (mt e)) (
+	Check (Expr · ∅)
+	(fun '(e, tt) => 
+    match (mt e) with
+    | None => false
+    | Some t' => mtypeCheck (pstep e) t'
+    end
+  ))).
 
-Definition test_prop_SinglePreserve_runner := (runLoop number_of_trials test_prop_SinglePreserve).
+Definition test_prop_SinglePreserve := (runLoop number_of_trials prop_SinglePreserve).
+(*! QuickProp test_prop_SinglePreserve. *)
 
-(*! QuickProp test_prop_SinglePreserve_runner. *)
-  
+Definition prop_MultiPreserve   :=
+	ForAllMaybe "e" (fun tt => gSized) (fun tt e => gSized) (fun tt => shrink) (fun tt => show) (
+  Implies (Expr · ∅) "isJust (mt e)" (fun '(e, tt) => isJust (mt e)) (
+	Check (Expr · ∅)
+	(fun '(e, tt) => 
+    match (mt e) with
+    | None => false
+    | Some t' => mtypeCheck (multistep 40 pstep e) t'
+    end
+  ))).
 
-Definition test_prop_MultiPreserve   :=
-	@ForAllMaybe _ ∅ _ "e" (fun tt => gSized) (fun tt n => (fun n => gSized)) (fun tt n => shrink n) (fun tt n => show n) (
-	@Predicate (Expr · ∅) Z
-	(fun '(e, tt) => (prop_MultiPreserve e, 0%Z))).
-
-Definition test_prop_MultiPreserve_runner := (runLoop number_of_trials test_prop_MultiPreserve).
-
-(*! QuickProp test_prop_MultiPreserve_runner. *)
-
-(*
-Derive (Arbitrary) for Typ.
-
-
-(* Fixpoint genTyp (s: nat) : G Typ :=
-  match s with
-  | 0 => ret TBool
-  | S s' => oneOf [
-    t1 <- genTyp s' ;;
-    t2 <- genTyp s' ;;
-    ret (TFun t1 t2) ;
-    ret TBool
-    ]
-  end.
-   *)
-
-(* #[export] Instance genArbitrary : GenSized Typ :=
-{|
- arbitrarySized x := genTyp x
-|}. *)
-
-Definition genTyp (s: nat) : G Typ := arbitrary.
-
-Fixpoint genOne (ctx: Ctx) (t: Typ) : G Expr :=
-  match t with
-  | TBool =>
-    b <- arbitrary ;;
-    ret (Bool b)
-  | TFun t1 t2 =>
-    t' <- genOne (t1 :: ctx) t2 ;;
-    ret (Abs t1 t')
-  end.
-
-
-Fixpoint genVar' (ctx: Ctx) (t: Typ) (p: nat) (r: list nat) : list nat :=
-  match ctx with
-  | nil => r
-  | t'::ctx' => if t == t' then genVar' ctx' t (p + 1) (p :: r)
-                else genVar' ctx' t (p + 1) r
-  end.
-
-
-Definition genVar (ctx: Ctx) (t: Typ) : list (G Expr) :=
-  let positions := genVar' ctx t 0 [] in
-  let tf := (fun n => ret (Var n)) in
-  map tf positions.
-
-
-Fixpoint genExactExpr (f: nat) (ctx: Ctx) (t: Typ) : G Expr :=
-  match f with
-  | O => oneOf_ (genOne ctx t) (genOne ctx t :: genVar ctx t)
-  | S f' =>
-    let abs : list (G Expr) := match t with
-              | TFun t1 t2 =>
-                [bindGen (genExactExpr f' (t1 :: ctx) t2) (fun t' => 
-                returnGen (Abs t1 t'))]
-              | _ => nil
-              end in
-    let one := genOne ctx t in
-    let app := 
-      t' <- genTyp f' ;;
-      e1 <- genExactExpr f' ctx (TFun t' t) ;;
-      e2 <- genExactExpr f' ctx t' ;;
-      ret (App e1 e2) in
-    let var := genVar ctx t in
-    
-    oneOf_ one ([one] ++ abs ++ [app] ++ var)
-  end.
-
-
-
-
-
-Definition genExpr (s: nat) : G Expr :=
-  t <- genTyp 3 ;;
-  genExactExpr s [] t
-.
-
-#[export] Instance arbitrarySizedExpr : GenSized Expr :=
-{|
-  arbitrarySized s := genExpr s
-|}.
-
-Definition gTyped := genExpr 5.
-
-Definition test_prop_SinglePreserve :=
-  forAll gTyped (fun (e: Expr) =>
-    prop_SinglePreserve e).
-
-(* QuickChick test_prop_SinglePreserve. *)
-
-Definition test_prop_MultiPreserve :=
-  forAll gTyped (fun (e: Expr) =>
-    prop_MultiPreserve e).
-
-(* QuickChick test_prop_MultiPreserve. *)
-
-
-
-
-
-
-*)
+Definition test_prop_MultiPreserve := (runLoop number_of_trials prop_MultiPreserve).
+(*! QuickProp test_prop_MultiPreserve. *)
